
\begin{proof} If $φ ≡ φ₁ ∨ φ₂$, we get for $i = 1, 2$,
\begin{equation*}
  \begin{bprooftree}
    \RightLabel{assume}
    \AxiomC{$Γ, φ_{i} ⊢ φ_{i}$}
    \RightLabel{by~ind.~hyp.}
    \UnaryInfC{$Γ ⊢ \fdist~φ_{i}$}
    \RightLabel{∨-intro$_{1,2}$}
    \UnaryInfC{$Γ, φ_{i} ⊢ \fdist~φ₁ ∨ \fdist~φ₂$}
    \RightLabel{Lemma~\ref{lem:dist-or}}
    \UnaryInfC{$Γ, φ_{i} ⊢ \fdist_{∨}(\fdist~φ₁ ∨ \fdist~φ₂)$}
    \end{bprooftree}
\end{equation*}

Then, by using the ∨-elim rule in the last derivation above, we
derive $Γ, φ₁ ∨ φ₂ ⟝ \fdist_{∨}(\fdist~φ₁ ∨ \fdist~φ₂)$ and the lemma
follows.
\end{proof}

\begin{equation}
\label{eq:strip-unfixed}
\begin{aligned}
&\hspace{.495mm}\fstripp : \Prop → \Prop\\
&\begin{array}{lll}
\fstripp &(φ₁ ∧ φ₂)     &= \fuh~(\fstripp~φ₁) ∧ \fuh~(φ₁ ⇒ \fstripp~φ₂)\\
\fstripp &(φ₁ ∨ φ₂)     &= \fuh~(¬ φ₁ ⇒ \fstripp~φ₂)\\
\fstripp &(φ₁ ⇒ φ₂)     &= \fuh~(φ₁ ⇒ \fstripp~φ₂)\\
\fstripp &(¬ (φ₁ ∧ φ₂)) &= \fuh~(φ₁ ⇒ \fstripp~¬ φ₂)\\
\fstripp &(¬ (φ₁ ∨ φ₂)) &= \fuh~(\fstripp~¬ φ₁) ∧ \fuh~(¬ φ₁ ⇒ \fstripp~¬ φ₂)\\
\fstripp &(¬ (φ₁ ⇒ φ₂)) &= \fuh~(\fstripp~φ₁) ∧ \fuh~(φ₁ ⇒ \fstripp~¬ φ₂)\\
\fstripp &(¬ ¬ φ₁)      &= \fuh~(\fstripp~φ₁)\\
\fstripp &(¬ ⊥)         &= ⊤\\
\fstripp &(¬ ⊤)         &= ⊥\\
\fstripp &φ             &= φ
\end{array}
\end{aligned}
\end{equation}

The function defined above is not a structural recursion function. Therefore,
we have reformulated it in~(\ref{eq:strip-fixed}) in order to solve such an
issue following the technique described in
Section~\ref{ssec:structural-recursion}.
